Renaming _a -> _partial

honeynet.v
@@ -43,9 +43,9 @@ Fixpoint fill_disk (level:nat) : Map_N_Byte :=
     end.
 Local Open Scope string.
 
-Definition honeynet_image_a : Disk := fill_disk 0%nat.
+Definition honeynet_image_partial : Disk := fill_disk 0%nat.
 (* All gunzip operations return the file mentioned *)
-Definition gunzipped_a : File := mkFile 
+Definition gunzipped_partial : File := mkFile 
   (FileIds.MockId (MN.elements gunzipped_23))
   1454080 (* uncompressed file size *)
   true
@@ -135,7 +135,7 @@ Definition file48284 := mkFile (Ext2Id 48284) 42736 true
                                (Some 984707102).
 
 Lemma lee_honeynet_file:
-  Timeline.isSound lee_timeline honeynet_image_a.
+  Timeline.isSound lee_timeline honeynet_image_partial.
 Proof.
   set (files := file23 :: file23 :: file30130 :: file30188 
                 :: file2056 :: file30191 :: file2055
@@ -155,11 +155,11 @@ Reflection - makes tactics smaller; makes proof terms smaller
 *)
 
 Lemma borland_honeynet_file:
-  (gunzip file23) = gunzipped_a 
-    -> borland_rootkit honeynet_image_a.
+  (gunzip file23) = gunzipped_partial 
+    -> borland_rootkit honeynet_image_partial.
   Proof.
     apply borland_reflection 
-      with (file := file23) (gunzipped := gunzipped_a)
+      with (file := file23) (gunzipped := gunzipped_partial)
            (filename1 := maliciousFileName1) 
            (filename2 := maliciousFileName2).
     vm_compute. reflexivity.
